otbn_model/code/montmul_lemmas.dfy
@@ -32,32 +32,33 @@ module montmul_lemmas {
 
     lemma r_r_inv_cancel_lemma(a: nat, rsa: rsa_params)
         requires rsa_params_inv(rsa);
-        ensures cong(a * rsa.R_INV * rsa.R, a, rsa.m);
+        ensures cong(a * rsa.R_INV * rsa.R, a, rsa.M);
     {
-        assert cong(rsa.R_INV * rsa.R, 1, rsa.m);
-        cong_mul_lemma_1(rsa.R_INV * rsa.R, 1, a, rsa.m);
+        assert cong(rsa.R_INV * rsa.R, 1, rsa.M);
+        cong_mul_lemma_1(rsa.R_INV * rsa.R, 1, a, rsa.M);
     }
     
     lemma r_r_inv_cancel_lemma_2(a: nat, b : nat, rsa: rsa_params)
         requires rsa_params_inv(rsa);
-        requires cong(a, b * rsa.R_INV * rsa.R, rsa.m);
-        ensures cong(a, b, rsa.m);
+        requires cong(a, b * rsa.R_INV * rsa.R, rsa.M);
+        ensures cong(a, b, rsa.M);
     {
-        assert cong(b * rsa.R_INV * rsa.R, b, rsa.m) by {
+        assert cong(b * rsa.R_INV * rsa.R, b, rsa.M) by {
             r_r_inv_cancel_lemma(b, rsa);
         }
         reveal cong();
     }
 
-    lemma montmul_inv_lemma_1(a_view: seq<uint256>,
+    lemma montmul_inv_lemma_1(
+        a_view: seq<uint256>,
         x: seq<uint256>,
         y: seq<uint256>,
         rsa: rsa_params)
     
         requires montmul_inv(a_view, x, NUM_WORDS, y, rsa);
-        ensures cong(to_nat(a_view), to_nat(x) * to_nat(y) * rsa.R_INV, rsa.m);
+        ensures cong(to_nat(a_view), to_nat(x) * to_nat(y) * rsa.R_INV, rsa.M);
     {
-        var m := rsa.m;
+        var m := rsa.M;
         var a := to_nat(a_view);
         assert x[..NUM_WORDS] == x;
 
